updates
Signed-off-by: Shaobo He <shaobohe@amazon.com>

cedar-lean/Cedar/Thm/TPE.lean
@@ -19,6 +19,8 @@ import Cedar.Spec
 import Cedar.Validation
 import Cedar.Thm.TPE.Input
 import Cedar.Thm
+import Cedar.Thm.Validation.TypedExpr
+import Cedar.Thm.Data
 
 namespace Cedar.Thm
 
@@ -28,24 +30,135 @@ open Cedar.Validation
 open Cedar.Thm.TPE
 open Cedar.Thm
 
-def TypedExpr.WellTyped : TypedExpr → Environment → Prop := sorry
-
-theorem well_typed_expr_cannot_go_wrong {env : Environment} {req : Request} {es : Entities} (x : TypedExpr) :
-  TypedExpr.WellTyped x env → ∃ v, EvaluatesTo x.toExpr req es v ∧ InstanceOfType v x.typeOf := by sorry
-
-theorem partialEvaluate_is_sound {c₁ c₂ : Capabilities}
+theorem partialEvaluate_is_sound
   (x : TypedExpr)
   (req₁ : Request)
   (es₁ : Entities)
   (req₂ : PartialRequest)
   (es₂ : PartialEntities)
   (env : Environment) :
-  TypedExpr.WellTyped x evn →
+  TypedExpr.WellTyped env x →
   RequestAndEntitiesMatchEnvironment env req₁ es₁ →
   PartialRequestAndEntitiesMatchEnvironment env req₂ es₂ →
   IsConsistent env req₁ es₁ req₂ es₂ →
-  (Spec.evaluate x.toExpr req₁ es₁).toOption = (Residual.evaluate (Cedar.TPE.evaluate x req₂ es₂) req e).toOption
+  (Spec.evaluate x.toExpr req₁ es₁).toOption = (Residual.evaluate (Cedar.TPE.evaluate x req₂ es₂) req₁ es₁).toOption
 := by
-  sorry
+  intro h₀ h₁ h₂ h₃
+  cases x
+  case and x₁ x₂ ty =>
+    unfold TypedExpr.WellTyped AndWellTyped at h₀
+    replace ⟨h₀, h₄⟩ := h₀
+    split at h₄
+    case _ ty₁ ty₂ heq =>
+      simp only [TPE.evaluate, TPE.and]
+      have h₅ := partialEvaluate_is_sound x₁ req₁ es₁ req₂ es₂ env h₀ h₁ h₂ h₃
+      split
+      case _ ty₃ _ _ _ _ heq₁ =>
+        rw [heq₁] at h₅
+        simp only [Residual.evaluate, Except.toOption] at h₅
+        have h₆ := well_typed_expr_cannot_go_wrong h₁ h₀
+        rw [heq] at h₆
+        cases h₆
+        rename_i v h₆
+        replace ⟨h₆, h₇⟩ := h₆
+        have h₇ := instance_of_ff_is_false h₇
+        rw [h₇] at h₆
+        simp only [EvaluatesTo] at h₆
+        rcases h₆ with h₆₁ | h₆₂ | h₆₃ | h₆₄
+        · rw [h₆₁] at h₅
+          simp only [reduceCtorEq] at h₅
+        · rw [h₆₂] at h₅
+          simp only [reduceCtorEq] at h₅
+        · rw [h₆₃] at h₅
+          simp only [reduceCtorEq] at h₅
+        · rw [h₆₄] at h₅
+          simp only [Option.some.injEq, Value.prim.injEq, Prim.bool.injEq, Bool.false_eq_true] at h₅
+      case _ ty₃ _ _ _ _ heq₁ =>
+        simp only [Residual.evaluate, Except.toOption]
+        split
+        · rename_i v heq₂
+          simp only [Option.some.injEq]
+          rw [heq₁] at h₅
+          simp [Residual.evaluate, Except.toOption] at h₅
+          split at h₅
+          have h₆ := well_typed_expr_cannot_go_wrong h₁ h₀
+          rw [heq] at h₆
+          cases h₆
+          rename_i h₆
+          replace ⟨h₆, h₇⟩ := h₆
+          have h₇ := instance_of_ff_is_false h₇
+          rw [h₇] at h₆
+          · rename_i _ _ _ heq₃ _ _
+            simp only [EvaluatesTo] at h₆
+            rw [heq₃] at h₆
+            simp only [reduceCtorEq, Except.ok.injEq, false_or] at h₆
+            rw [h₆] at heq₃
+            simp only [TypedExpr.toExpr, Spec.evaluate] at heq₂
+            rw [heq₃] at heq₂
+            simp only [Result.as, Coe.coe, Value.asBool, Bool.not_eq_eq_eq_not, Bool.not_true,
+              bind_pure_comp, Except.bind_ok, ↓reduceIte, Except.ok.injEq] at heq₂
+            symm at heq₂
+            exact heq₂
+          · cases h₅
+        · sorry
+      case _ ty₃ _ _ _ _ heq₁ =>
+        rw [heq₁] at h₅
+        simp only [Residual.evaluate, Except.toOption] at h₅
+        split at h₅
+        · cases h₅
+        · rename_i heq₂
+          simp only [Except.toOption, TypedExpr.toExpr, Spec.evaluate, Bool.not_eq_eq_eq_not,
+            Bool.not_true, bind_pure_comp, Residual.evaluate]
+          rw [heq₂]
+          simp only [Result.as, Except.bind_err]
+      case _ heq₁ _ _ _ =>
+        sorry
+      case _ =>
+        sorry
+    case _ _ bty₁ _ heq₁ heq₂ =>
+      simp only [TPE.evaluate, TPE.and]
+      split
+      · have h₅ := partialEvaluate_is_sound x₁ req₁ es₁ req₂ es₂ env h₀ h₁ h₂ h₃
+        rename_i heq₃
+        simp only [Except.toOption, heq₃, Residual.evaluate] at h₅
+        split at h₅
+        · rename_i heq₄
+          simp only [Option.some.injEq] at h₅
+          rw [h₅] at heq₄
+          simp only [TypedExpr.toExpr, Spec.evaluate, Bool.not_eq_eq_eq_not, Bool.not_true,
+            bind_pure_comp]
+          rw [heq₄]
+          simp [Result.as, Coe.coe, Value.asBool]
+          replace ⟨h₄, h₆⟩ := h₄
+          have h₇ := partialEvaluate_is_sound x₂ req₁ es₁ req₂ es₂ env h₄ h₁ h₂ h₃
+          have h₇ := to_option_p h₇
+
+
+
+          sorry
+        · sorry
+      · sorry
+      · sorry
+      · sorry
+      sorry
+    case _ =>
+      sorry
+    case _ => simp only at h₄
+  case lit => sorry
+  case var => sorry
+  case ite => sorry
+  case or => sorry
+  case unaryApp => sorry
+  case binaryApp => sorry
+  case getAttr => sorry
+  case hasAttr => sorry
+  case set => sorry
+  case record => sorry
+  case call => sorry
+
+
+
+
+
 
 end Cedar.Thm
