cedar-lean/Cedar/Thm/Data/Control.lean
@@ -61,3 +61,23 @@ theorem do_ok {res : Except ε α} {f : α → β} :
   (do let v ← res ; .ok (f v)) = .ok b ↔
   ∃ a, res = .ok a ∧ f a = b
 := by cases res <;> simp
+
+inductive ExceptEqₒ [DecidableEq α] : Except ε α → Except ε α → Prop
+| both_ok (x₁ x₂ : α) (h : x₁ = x₂) :
+  ExceptEqₒ (.ok x₁) (.ok x₂)
+| both_err (e₁ e₂ : ε) :
+  ExceptEqₒ (.error e₁) (.error e₂)
+
+theorem to_option_p [DecidableEq α] {res₁ : Except ε α} {res₂ : Except ε α} :
+  res₁.toOption = res₂.toOption → ExceptEqₒ res₁ res₂
+:= by
+  intro h
+  simp only [Except.toOption] at h
+  split at h <;> split at h
+  · case _ x₁ _ x₂ =>
+    simp only [Option.some.injEq] at h
+    exact ExceptEqₒ.both_ok x₁ x₂ h
+  · case _ => cases h
+  · case _ => cases h
+  · case _ e₁ _ e₂ =>
+      exact ExceptEqₒ.both_err e₁ e₂
